@prefix : <http://purl.org/hpi/patchr#> .
@prefix xsd: <http://www.w3.org/2001/XMLSchema#> .
@prefix owl: <http://www.w3.org/2002/07/owl#> .
@prefix rdfs: <http://www.w3.org/2000/01/rdf-schema#> .
@prefix rdf: <http://www.w3.org/1999/02/22-rdf-syntax-ns#> .
@prefix foaf: <http://xmlns.com/foaf/0.1/> .
@prefix void: <http://rdfs.org/ns/void> .
@prefix guo: <http://webr3.org/owl/guo#> .
@prefix prv: <http://purl.org/net/provenance/ns#> .
@prefix dc: <http://purl.org/dc/terms/> .

#######################################
### PatchR - Patch Request Ontology ###

<http://purl.org/hpi/patchr#>
	a owl:Ontology ;
	dc:creator <http://magnus.13mm.de> ;
	dc:creator <http://johannes.jhercher.de> ;
	dc:title "Patch Request Ontology"@en ;
	dc:description "The Patch Request Ontology provides a schema to describe desired changes in Linked Data. By wrapping the Graph Update Ontology (guo) patch requests can be formulated to add, modify or delete certain triples (or subgraphs) within a dataset."@en ;
    owl:versionInfo "Revision: 0.5" .

:Patch a owl:Class ;
	rdfs:comment "A patch is a request to add, change or delete certain triples (or subgraphs) within a dataset. A patch refers to an guo:UpdateInstruction. For convenient retrieval a patch should be described with provenance data, a patch type and a dataset it applies to."@en ;
	rdfs:isDefinedBy <http://purl.org/hpi/patchr#> ;
    rdfs:label "Patch"@en .

:PatchGroup a owl:Class ;
    rdfs:comment "A patch group is a collection of patches that apply to a common problem."@en ;
	rdfs:isDefinedBy <http://purl.org/hpi/patchr#> ;
    rdfs:label "PatchGroup"@en .

:DisjunctivePatchGroup a owl:Class ;
	rdfs:subClassOf :PatchGroup ;
	rdfs:comment "A disjunctive patch group is collection (alternative list) of patches where one member patch need to be applied to resolve the problem."@en ;
	rdfs:isDefinedBy <http://purl.org/hpi/patchr#> ;
    rdfs:label "DisjunctivePatchGroup"@en .

:ConjunctivePatchGroup a owl:Class ;
	rdfs:subClassOf :PatchGroup ;
	rdfs:comment "A conjunctive patch group is collection (list) of patches where all member patches need to be applied to the dataset to resolve the problem."@en ;
	rdfs:isDefinedBy <http://purl.org/hpi/patchr#> ;
    rdfs:label "ConjunctivePatchGroup"@en .

:PatchStatus a owl:Class ;
	rdfs:comment "Status of a patch can be either active or resolved."@en ;
	rdfs:isDefinedBy <http://purl.org/hpi/patchr#> ;
    rdfs:label "PatchStatus"@en .

### ObjectProperties ###

## deprecated, use prov:wasGeneratedBy instead
:provenance a owl:ObjectProperty ;
	rdfs:comment "Refers to the provenance context where this patch was created. Deprecated, use prov:wasGeneratedBy instead."@en;
	rdfs:domain [  a owl:Class ;
                   owl:unionOf ( :Patch
                                 :PatchGroup )
                ] ;
	rdfs:range prv:DataCreation ;
	rdfs:isDefinedBy <http://purl.org/hpi/patchr#> ;
    rdfs:label "provenance"@en .
	
:update a owl:FunctionalProperty, owl:ObjectProperty ;
	rdfs:comment "Refers to a guo:UpdateInstruction. There must be exactly one guo:UpdateInstruction per :Patch."@en ;
	rdfs:domain :Patch ;
	rdfs:range guo:UpdateInstruction ;
	rdfs:isDefinedBy <http://purl.org/hpi/patchr#> ;
    rdfs:label "update"@en .

:memberOf a owl:ObjectProperty ;
	rdfs:comment "Relates a Patch to a PatchGroup. A Patch may be part of multiple :PatchGroups."@en ;
	rdfs:domain :Patch ;
	rdfs:range :PatchGroup ;
	rdfs:isDefinedBy <http://purl.org/hpi/patchr#> ;
    rdfs:label "memberOf"@en .
	
:appliesTo a owl:ObjectProperty ;
	rdfs:comment "Refers to a void:Dataset to allow convenient selection of patches per dataset."@en ;
	rdfs:domain :Patch ;
	rdfs:range void:Dataset ;
	rdfs:isDefinedBy <http://purl.org/hpi/patchr#> ;
    rdfs:label "appliesTo"@en .

:advocate a owl:ObjectProperty ;
	rdfs:comment "Links agents who support, i.e. vote for, a :Patch. Each time a user creates a patch request, appropriate provenance information is generated."@en ;
	rdfs:domain :Patch ;
	rdfs:range foaf:Agent ;
	rdfs:isDefinedBy <http://purl.org/hpi/patchr#> ;
    rdfs:label "advocate"@en .
	
:criticiser a owl:ObjectProperty ;
	rdfs:comment "Links agents who disagree, i.e. vote against, a :Patch."@en ;
	rdfs:domain :Patch ;
	rdfs:range foaf:Agent ;
	rdfs:isDefinedBy <http://purl.org/hpi/patchr#> ;
    rdfs:label "criticiser"@en .

:patchType a owl:ObjectProperty ;
	rdfs:comment "Refers to a classification of the patch. There might be patch taxonomies from different applications that define the reason for a :Patch on their own. A :Patch may have multiple types."@en ;
	rdfs:domain :Patch ;
	rdfs:isDefinedBy <http://purl.org/hpi/patchr#> ;
    rdfs:label "patchType"@en .

:patchrService a owl:ObjectProperty ;
	rdfs:comment "Links a resource to the PatchR instance responsible for collecting patch requests."@en ;
	rdfs:isDefinedBy <http://purl.org/hpi/patchr#> ;
    rdfs:label "patchrService"@en .


### DatatypeProperties ###

## deprecated, use rdfs:comment instead
:comment a owl:DatatypeProperty ;
	rdfs:subPropertyOf rdfs:comment ;
	rdfs:comment "A comment on the patch. This is likely just an informal message a user wants to share when submitting a Patch. Deprecated, use rdfs:comment instead."@en ;
	rdfs:domain :Patch ;
	rdfs:range rdfs:Literal ;
	rdfs:isDefinedBy <http://purl.org/hpi/patchr#> ;
    rdfs:label "comment"@en .

# TODO: stati should be made resources instead of literals
:status a owl:DatatypeProperty ;
	rdfs:domain :Patch ;
	rdfs:comment "The status of the patch, might be \"resolved\" or \"open\"."@en ;
	rdfs:range rdfs:Literal ;
	rdfs:isDefinedBy <http://purl.org/hpi/patchr#> ;
    rdfs:label "status"@en .

:confidence a owl:DatatypeProperty ;
	rdfs:domain :Patch ;
	rdfs:comment "A confidence assigned by the creator of the patch, e.g. in case heuristic methods identified an inconsistency. This confidence must be expressed in the range of (0,1], whereas a high value means higher confidence and a value of 1 signifies absolute certainty."@en ;
	rdfs:range xsd:Double ;
	rdfs:isDefinedBy <http://purl.org/hpi/patchr#> ;
    rdfs:label "confidence"@en .

### Instances ###
:Active a :PatchStatus ;
	rdfs:comment "The patch has not been resolved."@en ;
	rdfs:isDefinedBy <http://purl.org/hpi/patchr#> ;
    rdfs:label "active"@en .

:Resolved a :PatchStatus ;
	rdfs:comment "The patch has been resolved."@en ;
	rdfs:isDefinedBy <http://purl.org/hpi/patchr#> ;
    rdfs:label "resolved"@en .

## Semantic Web Deployment (SWD) Tracker [http://www.w3.org/2006/07/SWD/wiki/IssuesProcess] knows:
## RAISED : Submitted, but not currently being discussed.
## OPEN : Actively being worked on, has an assigned owner, identified as Raised By in tracker.
## PENDING : Activity suspended, perhaps until some other controlling issue is resolved.
## POSTPONED : Activity suspended. Will not be resolved by this working group. Left for the next revision.
## CLOSED : Resolved.
## SUBSUMED : Allows some freedom in clearing up sets of issues. Tracker notes must identify the subsuming issue by URI.


###################################
### GUO - Graph Update Ontology ###
# 
# <http://webr3.org/owl/guo#>
#     dc:description "A lightweight RDF Graph update ontology suitable for per triple insertion and deletion in addition to graph merging and synchronisation instructions."@en ;
#     dc:title "RDF Graph Update Ontology"@en ;
#     a owl:Ontology, owl:Thing ;
#     owl:versionInfo "Revision: 0.02" .
# 
# <http://webr3.org/owl/guo#UpdateInstruction>
#     a owl:Class ;
#     rdfs:comment "The class of an RDF Update Instruction, an UpdateInstruction defines a instructions to be carried out by a GUO processor."@en ;
#     rdfs:isDefinedBy <http://webr3.org/owl/guo#> ;
#     rdfs:label "UpdateInstruction"@en .
# 
# <http://webr3.org/owl/guo#delete>
#     a owl:ObjectProperty ;
#     rdfs:comment "The delete property defines blank node or resource whose predicate and object values will be used to remove triples { target_subject predicate object } from target_graph(s) if specified"@en ;
#     rdfs:domain <http://webr3.org/owl/guo#UpdateInstruction> ;
#     rdfs:isDefinedBy <http://webr3.org/owl/guo#> ;
#     rdfs:label "delete"@en .
# 
# <http://webr3.org/owl/guo#insert>
#     a owl:ObjectProperty ;
#     rdfs:comment "The insert property defines a blank node or resource whose predicate and object values will be used to create new triples inside target_graph(s) if specified with target_subject"@en ;
#     rdfs:domain <http://webr3.org/owl/guo#UpdateInstruction> ;
#     rdfs:isDefinedBy <http://webr3.org/owl/guo#> ;
#     rdfs:label "insert"@en .
# 
# <http://webr3.org/owl/guo#merge>
#     a owl:ObjectProperty ;
#     rdfs:comment "The merge property defines a graph from which all triples should be merged in to the target_graph(s), unlike insert which works on a resource level rewriting subjects, merge works on a graph level where all triples are added \"as is\"."@en ;
#     rdfs:domain <http://webr3.org/owl/guo#UpdateInstruction> ;
#     rdfs:isDefinedBy <http://webr3.org/owl/guo#> ;
#     rdfs:label "merge"@en .
# 
# <http://webr3.org/owl/guo#target_graph>
#     a owl:ObjectProperty ;
#     rdfs:comment "Optional property of an UpdateInstruction which allows updates to apply only to the specified Named Graph(s)"@en ;
#     rdfs:domain <http://webr3.org/owl/guo#UpdateInstruction> ;
#     rdfs:isDefinedBy <http://webr3.org/owl/guo#> ;
#     rdfs:label "target graph"@en .
# 
# <http://webr3.org/owl/guo#target_subject>
#     a owl:ObjectProperty ;
#     rdfs:comment "the target_subject is a required property of all UpdateInstructions which specify an insert/delete statement, target_subject is combined with the predicate and object values from insert/delete nodes to form triples which are to be either inserted or deleted (optionally constrained to one or more target_graphs)"@en ;
#     rdfs:domain :UpdateInstruction ;
#     rdfs:isDefinedBy <http://webr3.org/owl/guo#> ;
#     rdfs:label "target subject"@en ;
#     rdfs:range owl:Thing .
# 
###################################